start of termination arguments
Signed-off-by: Craig Disselkoen <cdiss@amazon.com>

cedar-lean/Cedar/Spec/Value.lean
@@ -257,4 +257,74 @@ instance : LT Value where
 instance Value.decLt (a b : Value) : Decidable (a < b) :=
   if h : Value.lt a b then isTrue h else isFalse h
 
+/--
+  an alternate metric for "size" of a value, used in termination arguments
+-/
+def Value.size : Value -> Nat
+  | .prim _ => 1
+  | .set vs => 1 + (vs.elts.map Value.size).foldl Nat.add 0
+  | .record vs => 1 + (vs.values.map Value.size).foldl Nat.add 0
+  | .ext _ => 1
+decreasing_by all_goals sorry
+
+/--
+  lemma helpful in termination arguments
+-/
+theorem all_values_have_positive_size (v : Value) :
+  v.size > 0
+:= by
+  unfold Value.size
+  cases v <;> simp
+  case set s =>
+    generalize (s.elts.map Value.size).foldl Nat.add 0 = n
+    omega
+  case record m =>
+    generalize (m.values.map Value.size).foldl Nat.add 0 = n
+    omega
+
+/--
+  lemma helpful in termination arguments
+-/
+theorem Value.set_termination (v : Value) (vs : Set Value) :
+  v ∈ vs.elts → v.size < (Value.set vs).size
+:= by
+  intro h₁
+  unfold Value.size List.map
+  cases h₂ : vs.elts
+  case nil => simp [h₂] at h₁
+  case cons v' tail =>
+    cases v <;> simp
+    case prim p | ext x =>
+      -- our goal clearly follows from `all_values_have_positive_size`
+      -- and the fact that `Nat.add` is non-decreasing. But not sure
+      -- how to convince Lean
+      sorry
+    case set s =>
+      sorry
+    case record m =>
+      sorry
+
+/--
+  lemma helpful in termination arguments
+-/
+theorem Value.record_termination (v : Value) (m : Map Attr Value) :
+  v ∈ m.values → v.size < (Value.record m).size
+:= by
+  intro h₁
+  unfold Value.size List.map
+  cases h₂ : m.values
+  case nil => simp [h₂] at h₁
+  case cons v' tail =>
+    cases v <;> simp
+    case prim p | ext x =>
+      -- our goal clearly follows from `all_values_have_positive_size`
+      -- and the fact that `Nat.add` is non-decreasing. But not sure
+      -- how to convince Lean
+      sorry
+    case set s =>
+      sorry
+    case record m =>
+      sorry
+
+
 end Cedar.Spec
